src/program_proof/simplepb/pb_definitions.v
@@ -1,3 +1,124 @@
 From Perennial.program_proof Require Import grove_prelude.
-From Goose.github_com.mit_pdos.gokv.simplepb Require Import pb client config admin.
+From Goose.github_com.mit_pdos.gokv.simplepb Require Import pb.
 From Perennial.program_proof.grove_shared Require Import urpc_proof urpc_spec.
+
+Section pb_definitions.
+
+Context `{!heapGS Σ}.
+
+Record pb_system_names :=
+{
+
+}.
+
+Implicit Type γ : pb_system_names.
+
+Implicit Type σ : list (list u8).
+
+Definition own_Server (s:loc) γ : iProp Σ :=
+  ∃ (epoch:u64) (nextIndex:u64) (isPrimary:bool) (sm:loc) (clerks:Slice.t),
+  (* physical *)
+  "Hepoch" ∷ s ↦[pb.Server :: "epoch"] #epoch ∗
+  "HnextIndex" ∷ s ↦[pb.Server :: "nextIndex"] #nextIndex ∗
+  "HisPrimary" ∷ s ↦[pb.Server :: "isPrimary"] #isPrimary ∗
+  "Hsm" ∷ s ↦[pb.Server :: "sm"] #sm ∗
+  "Hclerks" ∷ s ↦[pb.Server :: "clerks"] (slice_val clerks) ∗
+
+  (* ghost *)
+
+  (* durable *)
+
+  (* primary-only *)
+  "#HareClerks" ∷ True
+.
+
+Definition pbN := nroot .@ "pb".
+
+Definition is_Server (s:loc) γ : iProp Σ :=
+  ∃ (mu:val),
+  "#Hmu" ∷ readonly (s ↦[pb.Server :: "mu"] mu) ∗
+  "#HmuInv" ∷ is_lock pbN mu (own_Server s γ).
+
+Record ApplyArgsC :=
+{
+  epoch : u64 ;
+  index : u64 ;
+  op : list u8 ;
+}.
+
+Definition has_encoding_ApplyArgs (encoded:list u8) (args:ApplyArgsC) : Prop.
+Admitted.
+
+Definition has_encoding_Error (encoded:list u8) (error:u64) : Prop.
+Admitted.
+
+Definition proposal_ptsto (epoch:u64) (σ:list (list u8)) : iProp Σ.
+Admitted.
+
+Definition accepted_lb (epoch:u64) (σ:list (list u8)) : iProp Σ.
+Admitted.
+
+Definition ApplyAsBackup_spec (encoded_args:list u8) Φ : iProp Σ :=
+  ∃ args σ,
+    ⌜has_encoding_ApplyArgs encoded_args args⌝ ∗
+    ⌜length σ = int.nat args.(index)⌝ ∗
+    ⌜last σ = Some args.(op)⌝ ∗
+    proposal_ptsto args.(epoch) σ ∗
+    (∀ error (reply:list u8),
+        ⌜has_encoding_Error reply error⌝ -∗
+        (if (decide (error = 0)) then accepted_lb args.(epoch) σ else True) -∗
+        Φ reply)
+.
+
+Lemma wp_Server__ApplyAsBackup (s:loc) (args_ptr:loc) γ (epoch index:u64) (op:list u8) op_sl :
+  is_Server s γ -∗
+  {{{
+        "HargEpoch" ∷ args_ptr ↦[pb.ApplyArgs :: "epoch"] #epoch ∗
+        "HargIndex" ∷ args_ptr ↦[pb.ApplyArgs :: "index"] #index ∗
+        "HargOp" ∷ args_ptr ↦[pb.ApplyArgs :: "op"] (slice_val op_sl) ∗
+        "HopSl" ∷ is_slice op_sl byteT 1 op
+        (* TODO:
+           ∗ epoch lower bound
+           ∗ (epoch, index) ↦ blah
+           ∗
+         *)
+  }}}
+    pb.Server__ApplyAsBackup #s #args_ptr
+  {{{
+        RET #(); True
+  }}}
+  .
+Proof.
+  iIntros "#HisSrv" (Φ) "!# Hpre HΦ".
+  iNamed "Hpre".
+  iNamed "HisSrv".
+  wp_call.
+  wp_loadField.
+  wp_apply (acquire_spec with "HmuInv").
+  iIntros "[Hlocked Hown]".
+  iNamed "Hown".
+  wp_pures.
+  wp_loadField.
+
+Admitted.
+
+Lemma wp_Server__Apply (s:loc) γ op_sl:
+  {{{
+        is_Server s γ
+  }}}
+    pb.Server__Apply #s (slice_val op_sl)
+  {{{
+        RET #(); True
+  }}}
+  .
+Proof.
+  iIntros (Φ) "#Hpre HΦ".
+  iNamed "Hpre".
+  wp_call.
+  wp_loadField.
+  wp_apply (acquire_spec with "HmuInv").
+  iIntros "[Hlocked Hown]".
+  iNamed "Hown".
+Admitted.
+
+End pb_definitions.
