src/goose_lang/trusted/github_com/tchajed/goose/internal/examples/trust_import/trusted_example.v
@@ -1,0 +1,12 @@
+From Perennial.goose_lang Require Import notation typing.
+
+Module trusted_example.
+  Section goose_lang.
+    Context {ext:ffi_syntax}.
+    Context {ext_tys: ext_types ext}.
+
+    Local Coercion Var' (s:string): expr := Var s.
+
+    Definition Foo: val := λ: <>, #().
+  End goose_lang.
+End trusted_example.
